src/Examples/Interval/CallString/Example_Interval_DG_CallString_K1.thy
@@ -312,7 +312,8 @@ proof (unfold_locales, unfold nest_cfg_compile,
   show ?case by (rule nest_finE)
 next
   case PP
-  show ?case by (rule nest_1_pp_st[unfolded nest_1_eqs_def])
+  show ?case
+    by (rule post_bounded_of_part_post_solution[OF nest_1_pp_st[unfolded nest_1_eqs_def]])
 next
   case (SgCov v c)
   show ?case using SgCov by (simp add: nest_gamma_def)
@@ -321,7 +322,7 @@ next
   show ?case using SgUncov by simp
 next
   case (Fwd u a v c)
-  show ?case using Fwd by (rule nest_fwd_closed_1)
+  show ?case using Fwd(1,3) by (rule nest_fwd_closed_1)
 next
   case IsBotBot show ?case by simp
 next
