src/Executable_Surface/CLI/Analysis_Run_Solver_Sound.thy
@@ -143,94 +143,94 @@ abbreviation int_cs_join_vars where
 subsection \<open>Entry state\<close>
 
 lemma interval_es_join_table:
-  assumes cov: "interval_es_join.terminates (declared_global p) p"
-      "ctx_vars_cover (prog_cfg p) (interval_es_join.ctx_succ (declared_global p) p) []
-         (interval_es_join.sol_vars (declared_global p) p)"
+  assumes wf: "wf_program_compile_input p"
+    and cov: "interval_es_join.terminates (declared_global p) p"
   shows "sound_table p (interval_es_join.result (declared_global p) p) interval_classify_check"
 proof (rule sound_table_of_activation
     [where R = "interval_es_join.admitted_contexts (declared_global p) p" and rc = "[]",
      OF _ _ _ interval_classify_check_proved interval_classify_check_refuted], goal_cases)
   case (1 u)
-  show ?case by (simp add: interval_es_join.entry_state_ltr_collect_eq_Union_of_cover [OF cov])
+  show ?case
+    by (simp add: interval_es_join.entry_state_ltr_collect_eq_Union_of_terminates [OF wf cov])
 next
   case (2 u ctx)
   show ?case
-    using interval_es_join.entry_state_activation_collect_sound_of_cover [OF cov]
+    using interval_es_join.entry_state_activation_collect_sound_of_terminates [OF wf cov]
     unfolding interval_es_join.gamma_reader_eq_lookup .
 next
   case 3
   show ?case
-    using interval_es_join.vars_finite_of_terminates [OF cov(1)]
+    using interval_es_join.vars_finite_of_terminates [OF cov]
     by (simp add: finite_analysis_result_def interval_es_join.result_def
         interval_es_join.sol_vars_def)
 qed
 
 lemma interval_es_po_table:
-  assumes cov: "interval_es_po.terminates (declared_global p) p"
-      "ctx_vars_cover (prog_cfg p) (interval_es_po.ctx_succ (declared_global p) p) []
-         (interval_es_po.sol_vars (declared_global p) p)"
+  assumes wf: "wf_program_compile_input p"
+    and cov: "interval_es_po.terminates (declared_global p) p"
   shows "sound_table p (interval_es_po.result (declared_global p) p) interval_classify_check"
 proof (rule sound_table_of_activation
     [where R = "interval_es_po.admitted_contexts (declared_global p) p" and rc = "[]",
      OF _ _ _ interval_classify_check_proved interval_classify_check_refuted], goal_cases)
   case (1 u)
-  show ?case by (simp add: interval_es_po.entry_state_ltr_collect_eq_Union_of_cover [OF cov])
+  show ?case
+    by (simp add: interval_es_po.entry_state_ltr_collect_eq_Union_of_terminates [OF wf cov])
 next
   case (2 u ctx)
   show ?case
-    using interval_es_po.entry_state_activation_collect_sound_of_cover [OF cov]
+    using interval_es_po.entry_state_activation_collect_sound_of_terminates [OF wf cov]
     unfolding interval_es_po.gamma_reader_eq_lookup .
 next
   case 3
   show ?case
-    using interval_es_po.vars_finite_of_terminates [OF cov(1)]
+    using interval_es_po.vars_finite_of_terminates [OF cov]
     by (simp add: finite_analysis_result_def interval_es_po.result_def
         interval_es_po.sol_vars_def)
 qed
 
 lemma interval_es_wpo_table:
-  assumes cov: "interval_es_wpo.terminates (declared_global p) p"
-      "ctx_vars_cover (prog_cfg p) (interval_es_wpo.ctx_succ (declared_global p) p) []
-         (interval_es_wpo.sol_vars (declared_global p) p)"
+  assumes wf: "wf_program_compile_input p"
+    and cov: "interval_es_wpo.terminates (declared_global p) p"
   shows "sound_table p (interval_es_wpo.result (declared_global p) p) interval_classify_check"
 proof (rule sound_table_of_activation
     [where R = "interval_es_wpo.admitted_contexts (declared_global p) p" and rc = "[]",
      OF _ _ _ interval_classify_check_proved interval_classify_check_refuted], goal_cases)
   case (1 u)
-  show ?case by (simp add: interval_es_wpo.entry_state_ltr_collect_eq_Union_of_cover [OF cov])
+  show ?case
+    by (simp add: interval_es_wpo.entry_state_ltr_collect_eq_Union_of_terminates [OF wf cov])
 next
   case (2 u ctx)
   show ?case
-    using interval_es_wpo.entry_state_activation_collect_sound_of_cover [OF cov]
+    using interval_es_wpo.entry_state_activation_collect_sound_of_terminates [OF wf cov]
     unfolding interval_es_wpo.gamma_reader_eq_lookup .
 next
   case 3
   show ?case
-    using interval_es_wpo.vars_finite_of_terminates [OF cov(1)]
+    using interval_es_wpo.vars_finite_of_terminates [OF cov]
     by (simp add: finite_analysis_result_def interval_es_wpo.result_def
         interval_es_wpo.sol_vars_def)
 qed
 
 lemma int_es_join_table:
-  assumes cov: "int_es_join_terminates (declared_global p) p"
-      "ctx_vars_cover (prog_cfg p) (int_es_join_ctx_succ (declared_global p) p) []
-         (int_es_join_vars (declared_global p) p)"
+  assumes wf: "wf_program_compile_input p"
+    and cov: "int_es_join_terminates (declared_global p) p"
   shows "sound_table p (analyse_int_entry_state_result p) int_classify_check"
 proof (rule sound_table_of_activation
     [where R = "int_es_join_ctx_rel (declared_global p) p" and rc = "[]",
      OF _ _ _ int_classify_check_proved int_classify_check_refuted], goal_cases)
   case (1 u)
-  show ?case by (simp add: analyse_int_entry_state_ltr_collect_eq_Union_of_cover [OF cov])
+  show ?case
+    by (simp add: analyse_int_entry_state_ltr_collect_eq_Union_of_terminates [OF wf cov])
 next
   case (2 u ctx)
   show ?case
-    using analyse_int_entry_state_sound_of_cover [OF cov]
+    using analyse_int_entry_state_sound_of_terminates [OF wf cov]
     unfolding analyse_int_entry_state_result_def analyse_int_entry_state_result_for_def
       analyse_int_entry_state_gamma_reader_eq_lookup .
 next
   case 3
   show ?case
-    using analyse_int_entry_state_vars_finite [OF cov(1)]
+    using analyse_int_entry_state_vars_finite [OF cov]
     by (simp add: finite_analysis_result_def analyse_int_entry_state_result_def
         analyse_int_entry_state_result_for_def
         routed_dg_pipeline.result_def routed_dg_pipeline.sol_vars_def)
@@ -239,9 +239,8 @@ qed
 subsection \<open>Call string\<close>
 
 lemma interval_cs_join_table:
-  assumes cov: "interval_cs_join_terminates k (declared_global p) p"
-      "ctx_vars_cover (prog_cfg p) (interval_cs_join_ctx_succ k (declared_global p) p) []
-         (interval_cs_join_vars k (declared_global p) p)"
+  assumes wf: "wf_program_compile_input p"
+    and cov: "interval_cs_join_terminates k (declared_global p) p"
   shows "sound_table p (interval_cs_join_result k (declared_global p) p) interval_classify_check"
 proof (rule sound_table_of_activation
     [where R = "call_context_rel_of_fun (\<lambda>u c t. cs_context k u c t)" and rc = "[]",
@@ -254,20 +253,20 @@ proof (rule sound_table_of_activation
 next
   case (2 u ctx)
   show ?case
-    using analyse_interval_call_string_sound_of_cover_join [OF cov, where s = "\<lambda>u c t. t"]
+    using analyse_interval_call_string_sound_of_terminates_join [OF wf cov,
+       where s = "\<lambda>u c t. t"]
     unfolding analyse_interval_call_string_gamma_reader_eq_lookup_join .
 next
   case 3
   show ?case
-    using analyse_interval_call_string_vars_finite_join [OF cov(1)]
+    using analyse_interval_call_string_vars_finite_join [OF cov]
     by (simp add: finite_analysis_result_def routed_dg_pipeline.result_def
         routed_dg_pipeline.sol_vars_def)
 qed
 
 lemma interval_cs_po_table:
-  assumes cov: "interval_cs_po_terminates k (declared_global p) p"
-      "ctx_vars_cover (prog_cfg p) (interval_cs_po_ctx_succ k (declared_global p) p) []
-         (interval_cs_po_vars k (declared_global p) p)"
+  assumes wf: "wf_program_compile_input p"
+    and cov: "interval_cs_po_terminates k (declared_global p) p"
   shows "sound_table p (interval_cs_po_result k (declared_global p) p) interval_classify_check"
 proof (rule sound_table_of_activation
     [where R = "call_context_rel_of_fun (\<lambda>u c t. cs_context k u c t)" and rc = "[]",
@@ -280,20 +279,20 @@ proof (rule sound_table_of_activation
 next
   case (2 u ctx)
   show ?case
-    using analyse_interval_call_string_sound_of_cover_po [OF cov, where s = "\<lambda>u c t. t"]
+    using analyse_interval_call_string_sound_of_terminates_po [OF wf cov,
+       where s = "\<lambda>u c t. t"]
     unfolding analyse_interval_call_string_gamma_reader_eq_lookup_po .
 next
   case 3
   show ?case
-    using analyse_interval_call_string_vars_finite_po [OF cov(1)]
+    using analyse_interval_call_string_vars_finite_po [OF cov]
     by (simp add: finite_analysis_result_def routed_dg_pipeline.result_def
         routed_dg_pipeline.sol_vars_def)
 qed
 
 lemma interval_cs_wpo_table:
-  assumes cov: "interval_cs_wpo_terminates k (declared_global p) p"
-      "ctx_vars_cover (prog_cfg p) (interval_cs_wpo_ctx_succ k (declared_global p) p) []
-         (interval_cs_wpo_vars k (declared_global p) p)"
+  assumes wf: "wf_program_compile_input p"
+    and cov: "interval_cs_wpo_terminates k (declared_global p) p"
   shows "sound_table p (interval_cs_wpo_result k (declared_global p) p) interval_classify_check"
 proof (rule sound_table_of_activation
     [where R = "call_context_rel_of_fun (\<lambda>u c t. cs_context k u c t)" and rc = "[]",
@@ -306,20 +305,20 @@ proof (rule sound_table_of_activation
 next
   case (2 u ctx)
   show ?case
-    using analyse_interval_call_string_sound_of_cover_wpo [OF cov, where s = "\<lambda>u c t. t"]
+    using analyse_interval_call_string_sound_of_terminates_wpo [OF wf cov,
+       where s = "\<lambda>u c t. t"]
     unfolding analyse_interval_call_string_gamma_reader_eq_lookup_wpo .
 next
   case 3
   show ?case
-    using analyse_interval_call_string_vars_finite_wpo [OF cov(1)]
+    using analyse_interval_call_string_vars_finite_wpo [OF cov]
     by (simp add: finite_analysis_result_def routed_dg_pipeline.result_def
         routed_dg_pipeline.sol_vars_def)
 qed
 
 lemma int_cs_join_table:
-  assumes cov: "int_cs_join_terminates k (declared_global p) p"
-      "ctx_vars_cover (prog_cfg p) (int_cs_join_ctx_succ k (declared_global p) p) []
-         (int_cs_join_vars k (declared_global p) p)"
+  assumes wf: "wf_program_compile_input p"
+    and cov: "int_cs_join_terminates k (declared_global p) p"
   shows "sound_table p (analyse_int_call_string_result k p) int_classify_check"
 proof (rule sound_table_of_activation
     [where R = "call_context_rel_of_fun (\<lambda>u c t. cs_context k u c t)" and rc = "[]",
@@ -331,17 +330,17 @@ proof (rule sound_table_of_activation
 next
   case (2 u ctx)
   show ?case
-    using analyse_int_call_string_sound_of_cover [OF cov, where s = "\<lambda>u c t. t"]
+    using analyse_int_call_string_sound_of_terminates [OF wf cov,
+       where s = "\<lambda>u c t. t"]
     unfolding analyse_int_call_string_result_def analyse_int_call_string_result_for_def
       analyse_int_call_string_gamma_reader_eq_lookup .
 next
   case 3
   show ?case
-    using analyse_int_call_string_vars_finite [OF cov(1)]
+    using analyse_int_call_string_vars_finite [OF cov]
     by (simp add: finite_analysis_result_def analyse_int_call_string_result_def
         analyse_int_call_string_result_for_def
         routed_dg_pipeline.result_def routed_dg_pipeline.sol_vars_def)
 qed
-
 end
 
